Expressions as dependent type.

barrier/barrier.v
@@ -1,10 +1,6 @@
-From heap_lang Require Export substitution notation.
+From heap_lang Require Export notation.
 
 Definition newbarrier : val := λ: <>, ref #0.
-Definition signal : val := λ: "x", "x" <- #1.
+Definition signal : val := λ: "x", '"x" <- #1.
 Definition wait : val :=
-  rec: "wait" "x" := if: !"x" = #1 then #() else "wait" "x".
-
-Instance newbarrier_closed : Closed newbarrier. Proof. solve_closed. Qed.
-Instance signal_closed : Closed signal. Proof. solve_closed. Qed.
-Instance wait_closed : Closed wait. Proof. solve_closed. Qed.
+  rec: "wait" "x" := if: !'"x" = #1 then #() else '"wait" '"x".
