heap_lang/lang.v
@@ -1,5 +1,5 @@
 From program_logic Require Export language.
-From prelude Require Export stringmap.
+From prelude Require Export strings.
 From prelude Require Import gmap.
 
 Module heap_lang.
@@ -17,41 +17,84 @@ Inductive bin_op : Set :=
 
 Inductive binder := BAnon | BNamed : string → binder.
 
+Definition cons_binder (mx : binder) (X : list string) : list string :=
+  match mx with BAnon => X | BNamed x => x :: X end.
+Infix ":b:" := cons_binder (at level 60, right associativity).
 Delimit Scope binder_scope with binder.
 Bind Scope binder_scope with binder.
+Instance binder_dec_eq (x1 x2 : binder) : Decision (x1 = x2).
+Proof. solve_decision. Defined.
 
-Inductive expr :=
+Instance set_unfold_cons_binder x mx X P :
+  SetUnfold (x ∈ X) P → SetUnfold (x ∈ mx :b: X) (BNamed x = mx ∨ P).
+Proof.
+  constructor. rewrite -(set_unfold (x ∈ X) P).
+  destruct mx; rewrite /= ?elem_of_cons; naive_solver.
+Qed.
+
+Class VarBound (x : string) (X : list string) :=
+  var_bound : bool_decide (x ∈ X).
+Hint Extern 0 (VarBound _ _) => vm_compute; exact I : typeclass_instances. 
+
+Instance var_bound_proof_irrel x X : ProofIrrel (VarBound x X).
+Proof. rewrite /VarBound. apply _. Qed.
+Instance set_unfold_var_bound x X P :
+  SetUnfold (x ∈ X) P → SetUnfold (VarBound x X) P.
+Proof.
+  constructor. by rewrite /VarBound bool_decide_spec (set_unfold (x ∈ X) P).
+Qed.
+
+Inductive expr (X : list string) :=
   (* Base lambda calculus *)
-  | Var (x : string)
-  | Rec (f x : binder) (e : expr)
-  | App (e1 e2 : expr)
+  | Var (x : string) `{VarBound x X}
+  | Rec (f x : binder) (e : expr (f :b: x :b: X))
+  | App (e1 e2 : expr X)
   (* Base types and their operations *)
   | Lit (l : base_lit)
-  | UnOp (op : un_op) (e : expr)
-  | BinOp (op : bin_op) (e1 e2 : expr)
-  | If (e0 e1 e2 : expr)
+  | UnOp (op : un_op) (e : expr X)
+  | BinOp (op : bin_op) (e1 e2 : expr X)
+  | If (e0 e1 e2 : expr X)
   (* Products *)
-  | Pair (e1 e2 : expr)
-  | Fst (e : expr)
-  | Snd (e : expr)
+  | Pair (e1 e2 : expr X)
+  | Fst (e : expr X)
+  | Snd (e : expr X)
   (* Sums *)
-  | InjL (e : expr)
-  | InjR (e : expr)
-  | Case (e0 : expr) (e1 : expr) (e2 : expr)
+  | InjL (e : expr X)
+  | InjR (e : expr X)
+  | Case (e0 : expr X) (e1 : expr X) (e2 : expr X)
   (* Concurrency *)
-  | Fork (e : expr)
+  | Fork (e : expr X)
   (* Heap *)
   | Loc (l : loc)
-  | Alloc (e : expr)
-  | Load (e : expr)
-  | Store (e1 : expr) (e2 : expr)
-  | Cas (e0 : expr) (e1 : expr) (e2 : expr).
+  | Alloc (e : expr X)
+  | Load (e : expr X)
+  | Store (e1 : expr X) (e2 : expr X)
+  | Cas (e0 : expr X) (e1 : expr X) (e2 : expr X).
 
 Bind Scope expr_scope with expr.
 Delimit Scope expr_scope with E.
+Arguments Var {_} _ {_}.
+Arguments Rec {_} _ _ _%E.
+Arguments App {_} _%E _%E.
+Arguments Lit {_} _.
+Arguments UnOp {_} _ _%E.
+Arguments BinOp {_} _ _%E _%E.
+Arguments If {_} _%E _%E _%E.
+Arguments Pair {_} _%E _%E.
+Arguments Fst {_} _%E.
+Arguments Snd {_} _%E.
+Arguments InjL {_} _%E.
+Arguments InjR {_} _%E.
+Arguments Case {_} _%E _%E _%E.
+Arguments Fork {_} _%E.
+Arguments Loc {_} _.
+Arguments Alloc {_} _%E.
+Arguments Load {_} _%E.
+Arguments Store {_} _%E _%E.
+Arguments Cas {_} _%E _%E _%E.
 
 Inductive val :=
-  | RecV (f x : binder) (e : expr) (* e should be closed *)
+  | RecV (f x : binder) (e : expr (f :b: x :b: []))
   | LitV (l : base_lit)
   | PairV (v1 v2 : val)
   | InjLV (v : val)
@@ -60,21 +103,13 @@ Inductive val :=
 
 Bind Scope val_scope with val.
 Delimit Scope val_scope with V.
+Arguments PairV _%V _%V.
+Arguments InjLV _%V.
+Arguments InjRV _%V.
 
-Global Instance base_lit_dec_eq (l1 l2 : base_lit) : Decision (l1 = l2).
-Proof. solve_decision. Defined.
-Global Instance un_op_dec_eq (op1 op2 : un_op) : Decision (op1 = op2).
-Proof. solve_decision. Defined.
-Global Instance bin_op_dec_eq (op1 op2 : bin_op) : Decision (op1 = op2).
-Proof. solve_decision. Defined.
-Global Instance binder_dec_eq (x1 x2 : binder) : Decision (x1 = x2).
-Proof. solve_decision. Defined.
-Global Instance expr_dec_eq (e1 e2 : expr) : Decision (e1 = e2).
-Proof. solve_decision. Defined.
-Global Instance val_dec_eq (v1 v2 : val) : Decision (v1 = v2).
-Proof. solve_decision. Defined.
+Definition signal : val := RecV BAnon (BNamed "x") (Store (Var "x") (Lit (LitInt 1))).
 
-Fixpoint of_val (v : val) : expr :=
+Fixpoint of_val (v : val) : expr [] :=
   match v with
   | RecV f x e => Rec f x e
   | LitV l => Lit l
@@ -83,7 +118,8 @@ Fixpoint of_val (v : val) : expr :=
   | InjRV v => InjR (of_val v)
   | LocV l => Loc l
   end.
-Fixpoint to_val (e : expr) : option val :=
+
+Fixpoint to_val (e : expr []) : option val :=
   match e with
   | Rec f x e => Some (RecV f x e)
   | Lit l => Some (LitV l)
@@ -99,30 +135,30 @@ Definition state := gmap loc val.
 
 (** Evaluation contexts *)
 Inductive ectx_item :=
-  | AppLCtx (e2 : expr)
+  | AppLCtx (e2 : expr [])
   | AppRCtx (v1 : val)
   | UnOpCtx (op : un_op)
-  | BinOpLCtx (op : bin_op) (e2 : expr)
+  | BinOpLCtx (op : bin_op) (e2 : expr [])
   | BinOpRCtx (op : bin_op) (v1 : val)
-  | IfCtx (e1 e2 : expr)
-  | PairLCtx (e2 : expr)
+  | IfCtx (e1 e2 : expr [])
+  | PairLCtx (e2 : expr [])
   | PairRCtx (v1 : val)
   | FstCtx
   | SndCtx
   | InjLCtx
   | InjRCtx
-  | CaseCtx (e1 : expr) (e2 : expr)
+  | CaseCtx (e1 : expr []) (e2 : expr [])
   | AllocCtx
   | LoadCtx
-  | StoreLCtx (e2 : expr)
+  | StoreLCtx (e2 : expr [])
   | StoreRCtx (v1 : val)
-  | CasLCtx (e1 : expr)  (e2 : expr)
-  | CasMCtx (v0 : val) (e2 : expr)
+  | CasLCtx (e1 : expr [])  (e2 : expr [])
+  | CasMCtx (v0 : val) (e2 : expr [])
   | CasRCtx (v0 : val) (v1 : val).
 
 Notation ectx := (list ectx_item).
 
-Definition fill_item (Ki : ectx_item) (e : expr) : expr :=
+Definition fill_item (Ki : ectx_item) (e : expr []) : expr [] :=
   match Ki with
   | AppLCtx e2 => App e e2
   | AppRCtx v1 => App (of_val v1) e
@@ -145,36 +181,83 @@ Definition fill_item (Ki : ectx_item) (e : expr) : expr :=
   | CasMCtx v0 e2 => Cas (of_val v0) e e2
   | CasRCtx v0 v1 => Cas (of_val v0) (of_val v1) e
   end.
-Definition fill (K : ectx) (e : expr) : expr := fold_right fill_item e K.
+Definition fill (K : ectx) (e : expr []) : expr [] := fold_right fill_item e K.
 
 (** Substitution *)
 (** We have [subst' e BAnon v = e] to deal with anonymous binders *)
-Fixpoint subst (e : expr) (x : string) (v : val) : expr :=
-  match e with
-  | Var y => if decide (x = y) then of_val v else Var y
-  | Rec f y e =>
-     Rec f y (if decide (BNamed x ≠ f ∧ BNamed x ≠ y) then subst e x v else e)
-  | App e1 e2 => App (subst e1 x v) (subst e2 x v)
+Lemma wexpr_rec_prf {X Y} (H : X `included` Y) {f x} :
+  f :b: x :b: X `included` f :b: x :b: Y.
+Proof. set_solver. Qed.
+
+Program Fixpoint wexpr {X Y} (H : X `included` Y) (e : expr X) : expr Y :=
+  match e return expr Y with
+  | Var x _ => @Var _ x _
+  | Rec f x e => Rec f x (wexpr (wexpr_rec_prf H) e)
+  | App e1 e2 => App (wexpr H e1) (wexpr H e2)
   | Lit l => Lit l
-  | UnOp op e => UnOp op (subst e x v)
-  | BinOp op e1 e2 => BinOp op (subst e1 x v) (subst e2 x v)
-  | If e0 e1 e2 => If (subst e0 x v) (subst e1 x v) (subst e2 x v)
-  | Pair e1 e2 => Pair (subst e1 x v) (subst e2 x v)
-  | Fst e => Fst (subst e x v)
-  | Snd e => Snd (subst e x v)
-  | InjL e => InjL (subst e x v)
-  | InjR e => InjR (subst e x v)
-  | Case e0 e1 e2 =>
-     Case (subst e0 x v) (subst e1 x v) (subst e2 x v)
-  | Fork e => Fork (subst e x v)
+  | UnOp op e => UnOp op (wexpr H e)
+  | BinOp op e1 e2 => BinOp op (wexpr H e1) (wexpr H e2)
+  | If e0 e1 e2 => If (wexpr H e0) (wexpr H e1) (wexpr H e2)
+  | Pair e1 e2 => Pair (wexpr H e1) (wexpr H e2)
+  | Fst e => Fst (wexpr H e)
+  | Snd e => Snd (wexpr H e)
+  | InjL e => InjL (wexpr H e)
+  | InjR e => InjR (wexpr H e)
+  | Case e0 e1 e2 => Case (wexpr H e0) (wexpr H e1) (wexpr H e2)
+  | Fork e => Fork (wexpr H e)
   | Loc l => Loc l
-  | Alloc e => Alloc (subst e x v)
-  | Load e => Load (subst e x v)
-  | Store e1 e2 => Store (subst e1 x v) (subst e2 x v)
-  | Cas e0 e1 e2 => Cas (subst e0 x v) (subst e1 x v) (subst e2 x v)
+  | Alloc e => Alloc (wexpr H e)
+  | Load  e => Load (wexpr H e)
+  | Store e1 e2 => Store (wexpr H e1) (wexpr H e2)
+  | Cas e0 e1 e2 => Cas (wexpr H e0) (wexpr H e1) (wexpr H e2)
   end.
-Definition subst' (e : expr) (mx : binder) (v : val) : expr :=
-  match mx with BNamed x => subst e x v | BAnon => e end.
+Solve Obligations with set_solver.
+
+Definition of_val' {X} (v : val) : expr X := wexpr (included_nil _) (of_val v).
+
+Lemma wsubst_rec_true_prf {X Y x} (H : X `included` x :: Y) {f y}
+    (Hfy :BNamed x ≠ f ∧ BNamed x ≠ y) :
+  f :b: y :b: X `included` x :: f :b: y :b: Y.
+Proof. set_solver. Qed.
+Lemma wsubst_rec_false_prf {X Y x} (H : X `included` x :: Y) {f y}
+    (Hfy : ¬(BNamed x ≠ f ∧ BNamed x ≠ y)) :
+  f :b: y :b: X `included` f :b: y :b: Y.
+Proof. move: Hfy=>/not_and_l [/dec_stable|/dec_stable]; set_solver. Qed.
+
+Program Fixpoint wsubst {X Y} (x : string) (es : expr [])
+    (H : X `included` x :: Y) (e : expr X)  : expr Y :=
+  match e return expr Y with
+  | Var y _ => if decide (x = y) then wexpr _ es else @Var _ y _
+  | Rec f y e =>
+     Rec f y $ match decide (BNamed x ≠ f ∧ BNamed x ≠ y) return _ with
+               | left Hfy => wsubst x es (wsubst_rec_true_prf H Hfy) e
+               | right Hfy => wexpr (wsubst_rec_false_prf H Hfy) e
+               end
+  | App e1 e2 => App (wsubst x es H e1) (wsubst x es H e2)
+  | Lit l => Lit l
+  | UnOp op e => UnOp op (wsubst x es H e)
+  | BinOp op e1 e2 => BinOp op (wsubst x es H e1) (wsubst x es H e2)
+  | If e0 e1 e2 => If (wsubst x es H e0) (wsubst x es H e1) (wsubst x es H e2)
+  | Pair e1 e2 => Pair (wsubst x es H e1) (wsubst x es H e2)
+  | Fst e => Fst (wsubst x es H e)
+  | Snd e => Snd (wsubst x es H e)
+  | InjL e => InjL (wsubst x es H e)
+  | InjR e => InjR (wsubst x es H e)
+  | Case e0 e1 e2 =>
+     Case (wsubst x es H e0) (wsubst x es H e1) (wsubst x es H e2)
+  | Fork e => Fork (wsubst x es H e)
+  | Loc l => Loc l
+  | Alloc e => Alloc (wsubst x es H e)
+  | Load e => Load (wsubst x es H e)
+  | Store e1 e2 => Store (wsubst x es H e1) (wsubst x es H e2)
+  | Cas e0 e1 e2 => Cas (wsubst x es H e0) (wsubst x es H e1) (wsubst x es H e2)
+  end.
+Solve Obligations with set_solver.
+
+Definition subst {X} (x : string) (es : expr []) (e : expr (x :: X)) : expr X :=
+  wsubst x es (λ z, id) e.
+Definition subst' {X} (mx : binder) (es : expr []) : expr (mx :b: X) → expr X :=
+  match mx with BNamed x => subst x es | BAnon => id end.
 
 (** The stepping relation *)
 Definition un_op_eval (op : un_op) (l : base_lit) : option base_lit :=
@@ -194,11 +277,11 @@ Definition bin_op_eval (op : bin_op) (l1 l2 : base_lit) : option base_lit :=
   | _, _, _ => None
   end.
 
-Inductive head_step : expr → state → expr → state → option expr → Prop :=
-  | BetaS f x e1 e2 v2 σ :
+Inductive head_step : expr [] → state → expr [] → state → option (expr []) → Prop :=
+  | BetaS f x e1 e2 v2 e' σ :
      to_val e2 = Some v2 →
-     head_step (App (Rec f x e1) e2) σ
-       (subst' (subst' e1 f (RecV f x e1)) x v2) σ None
+     e' = subst' x (of_val v2) (subst' f (Rec f x e1) e1) →
+     head_step (App (Rec f x e1) e2) σ e' σ None
   | UnOpS op l l' σ :
      un_op_eval op l = Some l' → 
      head_step (UnOp op (Lit l)) σ (Lit l') σ None
@@ -242,7 +325,7 @@ Inductive head_step : expr → state → expr → state → option expr → Prop
      head_step (Cas (Loc l) e1 e2) σ (Lit $ LitBool true) (<[l:=v2]>σ) None.
 
 (** Atomic expressions *)
-Definition atomic (e: expr) : Prop :=
+Definition atomic (e: expr []) : Prop :=
   match e with
   | Alloc e => is_Some (to_val e)
   | Load e => is_Some (to_val e)
@@ -255,11 +338,69 @@ Definition atomic (e: expr) : Prop :=
 
 (** Close reduction under evaluation contexts.
 We could potentially make this a generic construction. *)
-Inductive prim_step
-    (e1 : expr) (σ1 : state) (e2 : expr) (σ2: state) (ef: option expr) : Prop :=
+Inductive prim_step (e1 : expr []) (σ1 : state)
+    (e2 : expr []) (σ2: state) (ef: option (expr [])) : Prop :=
   Ectx_step K e1' e2' :
     e1 = fill K e1' → e2 = fill K e2' →
     head_step e1' σ1 e2' σ2 ef → prim_step e1 σ1 e2 σ2 ef.
+
+(** Substitution *)
+Lemma var_proof_irrel X x H1 H2 : @Var X x H1 = @Var X x H2.
+Proof. f_equal. by apply (proof_irrel _). Qed.
+
+Lemma wexpr_id X (H : X `included` X) e : wexpr H e = e.
+Proof. induction e; f_equal/=; auto. by apply (proof_irrel _). Qed.
+Lemma wexpr_proof_irrel X Y (H1 H2 : X `included` Y) e : wexpr H1 e = wexpr H2 e.
+Proof.
+  revert Y H1 H2; induction e; simpl; auto using var_proof_irrel with f_equal.
+Qed.
+Lemma wexpr_wexpr X Y Z (H1 : X `included` Y) (H2 : Y `included` Z) H3 e :
+  wexpr H2 (wexpr H1 e) = wexpr H3 e.
+Proof.
+  revert Y Z H1 H2 H3.
+  induction e; simpl; auto using var_proof_irrel with f_equal.
+Qed.
+Lemma wexpr_wexpr' X Y Z (H1 : X `included` Y) (H2 : Y `included` Z) e :
+  wexpr H2 (wexpr H1 e) = wexpr (transitivity H1 H2) e.
+Proof. apply wexpr_wexpr. Qed.
+
+Lemma wsubst_proof_irrel X Y x es (H1 H2 : X `included` x :: Y) e :
+  wsubst x es H1 e = wsubst x es H2 e.
+Proof.
+  revert Y H1 H2; induction e; simpl; intros; repeat case_decide;
+    auto using var_proof_irrel, wexpr_proof_irrel with f_equal.
+Qed.
+Lemma wexpr_wsubst X Y Z x es (H1: X `included` x::Y) (H2: Y `included` Z) H3 e:
+  wexpr H2 (wsubst x es H1 e) = wsubst x es H3 e.
+Proof.
+  revert Y Z H1 H2 H3.
+  induction e; intros; repeat (case_decide || simplify_eq/=);
+    auto using var_proof_irrel, wexpr_wexpr with f_equal.
+Qed.
+Lemma wsubst_wexpr X Y Z x es (H1: X `included` Y) (H2: Y `included` x::Z) H3 e:
+  wsubst x es H2 (wexpr H1 e) = wsubst x es H3 e.
+Proof.
+  revert Y Z H1 H2 H3.
+  induction e; intros; repeat (case_decide || simplify_eq/=);
+    auto using var_proof_irrel, wexpr_wexpr with f_equal.
+Qed.
+Lemma wsubst_wexpr' X Y Z x es (H1: X `included` Y) (H2: Y `included` x::Z) e:
+  wsubst x es H2 (wexpr H1 e) = wsubst x es (transitivity H1 H2) e.
+Proof. apply wsubst_wexpr. Qed.
+
+Lemma wsubst_closed X Y x es (H1 : X `included` x :: Y) H2 (e : expr X) :
+  x ∉ X → wsubst x es H1 e = wexpr H2 e.
+Proof.
+  revert Y H1 H2.
+  induction e; intros; repeat (case_decide || simplify_eq/=);
+    auto using var_proof_irrel, wexpr_proof_irrel with f_equal set_solver.
+  exfalso; set_solver.
+Qed.
+Lemma wsubst_closed_nil x es H (e : expr []) : wsubst x es H e = e.
+Proof.
+  rewrite -{2}(wexpr_id _ (reflexivity []) e).
+  apply wsubst_closed, not_elem_of_nil.
+Qed.
 
 (** Basic properties about the language *)
 Lemma to_of_val v : to_val (of_val v) = Some v.
@@ -267,7 +408,13 @@ Proof. by induction v; simplify_option_eq. Qed.
 
 Lemma of_to_val e v : to_val e = Some v → of_val v = e.
 Proof.
-  revert v; induction e; intros; simplify_option_eq; auto with f_equal.
+  revert e v. cut (∀ X (e : expr X) (H : X = ∅) v,
+    to_val (eq_rect _ expr e _ H) = Some v → of_val v = eq_rect _ expr e _ H).
+  { intros help e v. apply (help ∅ e eq_refl). }
+  intros X e; induction e; intros HX ??; simplify_option_eq;
+    repeat match goal with
+    | IH : ∀ _ : ∅ = ∅, _ |- _ => specialize (IH eq_refl); simpl in IH
+    end; auto with f_equal.
 Qed.
 
 Instance: Inj (=) (=) of_val.
@@ -316,7 +463,7 @@ Qed.
 Lemma atomic_head_step e1 σ1 e2 σ2 ef :
   atomic e1 → head_step e1 σ1 e2 σ2 ef → is_Some (to_val e2).
 Proof.
-  destruct 2; simpl; rewrite ?to_of_val; try by eauto.
+  destruct 2; simpl; rewrite ?to_of_val; try by eauto. subst.
   unfold subst'; repeat (case_match || contradiction || simplify_eq/=); eauto.
 Qed.
 
@@ -363,92 +510,53 @@ Lemma alloc_fresh e v σ :
   to_val e = Some v → head_step (Alloc e) σ (Loc l) (<[l:=v]>σ) None.
 Proof. by intros; apply AllocS, (not_elem_of_dom (D:=gset _)), is_fresh. Qed.
 
-(** Closed expressions *)
-Definition of_binder (mx : binder) : stringset :=
-  match mx with BAnon => ∅ | BNamed x => {[ x ]} end.
-Lemma elem_of_of_binder x mx: x ∈ of_binder mx ↔ mx = BNamed x.
-Proof. destruct mx; set_solver. Qed.
-Global Instance set_unfold_of_binder (mx : binder) x :
-  SetUnfold (x ∈ of_binder mx) (mx = BNamed x).
-Proof. constructor; destruct mx; set_solver. Qed.
+(** Equality stuff *)
+Instance base_lit_dec_eq (l1 l2 : base_lit) : Decision (l1 = l2).
+Proof. solve_decision. Defined.
+Instance un_op_dec_eq (op1 op2 : un_op) : Decision (op1 = op2).
+Proof. solve_decision. Defined.
+Instance bin_op_dec_eq (op1 op2 : bin_op) : Decision (op1 = op2).
+Proof. solve_decision. Defined.
 
-Fixpoint is_closed (X : stringset) (e : expr) : bool :=
-  match e with
-  | Var x => bool_decide (x ∈ X)
-  | Rec f y e => is_closed (of_binder f ∪ of_binder y ∪ X) e
-  | App e1 e2 => is_closed X e1 && is_closed X e2
-  | Lit l => true
-  | UnOp _ e => is_closed X e
-  | BinOp _ e1 e2 => is_closed X e1 && is_closed X e2
-  | If e0 e1 e2 => is_closed X e0 && is_closed X e1 && is_closed X e2
-  | Pair e1 e2 => is_closed X e1 && is_closed X e2
-  | Fst e => is_closed X e
-  | Snd e => is_closed X e
-  | InjL e => is_closed X e
-  | InjR e => is_closed X e
-  | Case e0 e1 e2 => is_closed X e0 && is_closed X e1 && is_closed X e2
-  | Fork e => is_closed X e
-  | Loc l => true
-  | Alloc e => is_closed X e
-  | Load e => is_closed X e
-  | Store e1 e2 => is_closed X e1 && is_closed X e2
-  | Cas e0 e1 e2 => is_closed X e0 && is_closed X e1 && is_closed X e2
+Fixpoint expr_beq {X Y} (e : expr X) (e' : expr Y) : bool :=
+  match e, e' with
+  | Var x _, Var x' _ => bool_decide (x = x')
+  | Rec f x e, Rec f' x' e' =>
+     bool_decide (f = f') && bool_decide (x = x') && expr_beq e e'
+  | App e1 e2, App e1' e2' | Pair e1 e2, Pair e1' e2' |
+    Store e1 e2, Store e1' e2' => expr_beq e1 e1' && expr_beq e2 e2'
+  | Lit l, Lit l' => bool_decide (l = l')
+  | UnOp op e, UnOp op' e' => bool_decide (op = op') && expr_beq e e'
+  | BinOp op e1 e2, BinOp op' e1' e2' =>
+     bool_decide (op = op') && expr_beq e1 e1' && expr_beq e2 e2'
+  | If e0 e1 e2, If e0' e1' e2' | Case e0 e1 e2, Case e0' e1' e2' |
+    Cas e0 e1 e2, Cas e0' e1' e2' =>
+     expr_beq e0 e0' && expr_beq e1 e1' && expr_beq e2 e2'
+  | Fst e, Fst e' | Snd e, Snd e' | InjL e, InjL e' | InjR e, InjR e' |
+    Fork e, Fork e' | Alloc e, Alloc e' | Load e, Load e' => expr_beq e e'
+  | Loc l, Loc l' => bool_decide (l = l')
+  | _, _ => false
   end.
-Class Closed (e : expr) := closed : ∀ x v, subst e x v = e.
-
-Lemma is_closed_subst_same X e x v : is_closed X e → x ∉ X → subst e x v = e.
+Lemma expr_beq_correct {X} (e1 e2 : expr X) : expr_beq e1 e2 ↔ e1 = e2.
 Proof.
-  revert X. induction e; simpl;
-    repeat case_decide; naive_solver eauto with f_equal set_solver.
+  split.
+  * revert e2; induction e1; intros [] * ?; simpl in *;
+      destruct_and?; subst; repeat f_equal/=; auto; try apply proof_irrel.
+  * intros ->. induction e2; naive_solver.
 Qed.
-Lemma is_closed_Closed e : is_closed ∅ e → Closed e.
-Proof. intros ? x v. by eapply is_closed_subst_same, not_elem_of_empty. Qed.
-
-Ltac solve_closed := apply is_closed_Closed; vm_compute; exact I.
-
-Lemma is_closed_weaken X Y e : is_closed X e → X ⊆ Y → is_closed Y e.
+Instance expr_dec_eq {X} (e1 e2 : expr X) : Decision (e1 = e2).
 Proof.
-  revert X Y.
-  induction e; simpl; intros; naive_solver eauto with f_equal set_solver.
-Qed.
-
-Lemma is_closed_fill_item X Ki e : is_closed X (fill_item Ki e) → is_closed X e.
-Proof. destruct Ki; rewrite /= ?andb_True; tauto. Qed.
-Lemma is_closed_fill X K e : is_closed X (fill K e) → is_closed X e.
-Proof. induction K; simpl; eauto using is_closed_fill_item. Qed.
-
-Lemma is_closed_subst X e x v :
-  is_closed ({[x]} ∪ X) e → is_closed ∅ (of_val v) → is_closed X (subst e x v).
+ refine (cast_if (decide (expr_beq e1 e2))); by rewrite -expr_beq_correct.
+Defined.
+Instance val_dec_eq (v1 v2 : val) : Decision (v1 = v2).
 Proof.
-  revert X. elim: e; simpl; try by intros; destruct_and?; split_and?; auto.
-  - intros y X; rewrite bool_decide_spec=>??.
-    case_decide; subst; last set_solver.
-    eauto using is_closed_weaken with set_solver.
-  - intros f y e IH X ??. case_decide as Hx.
-    + apply IH; clear IH; eauto using is_closed_weaken with set_solver.
-    + clear IH; apply not_and_l in Hx;
-        destruct Hx as [Hx|Hx]; apply dec_stable in Hx; subst;
-        eauto using is_closed_weaken with set_solver.
-Qed.
-Lemma is_closed_subst' X e x v :
-  is_closed (of_binder x ∪ X) e → is_closed ∅ (of_val v) →
-  is_closed X (subst' e x v).
-Proof. destruct x; rewrite /= ?left_id_L; auto using is_closed_subst. Qed.
-Lemma is_closed_head_step e1 σ1 e2 σ2 ef :
-  (* for load, the state should be closed *)
-  match e1 with Load _ => False | _ => True end →
-  head_step e1 σ1 e2 σ2 ef → is_closed ∅ e1 → is_closed ∅ e2.
-Proof.
-  destruct 2; rewrite /= ?andb_True; try
-    match goal with H : to_val _ = _ |- _ => apply of_to_val in H; subst end;
-    try tauto.
-  intros [??]. repeat apply is_closed_subst'; rewrite /= ?assoc_L; auto.
-Qed.
+ refine (cast_if (decide (of_val v1 = of_val v2))); abstract naive_solver.
+Defined.
 End heap_lang.
 
 (** Language *)
 Program Canonical Structure heap_lang : language := {|
-  expr := heap_lang.expr; val := heap_lang.val; state := heap_lang.state;
+  expr := heap_lang.expr []; val := heap_lang.val; state := heap_lang.state;
   of_val := heap_lang.of_val; to_val := heap_lang.to_val;
   atomic := heap_lang.atomic; prim_step := heap_lang.prim_step;
 |}.
