heap_lang/tests.v
@@ -4,21 +4,15 @@ From heap_lang Require Import wp_tactics heap notation.
 Import uPred.
 
 Section LangTests.
-  Definition add := (#21 + #21)%E.
+  Definition add : expr [] := (#21 + #21)%E.
   Goal ∀ σ, prim_step add σ (#42) σ None.
   Proof. intros; do_step done. Qed.
-  Definition rec_app : expr := ((rec: "f" "x" := "f" "x") #0).
+  Definition rec_app : expr [] := ((rec: "f" "x" := '"f" '"x") #0)%E.
   Goal ∀ σ, prim_step rec_app σ rec_app σ None.
-  Proof.
-    intros. rewrite /rec_app. (* FIXME: do_step does not work here *)
-    by eapply (Ectx_step  _ _ _ _ _ []), (BetaS _ _ _ _ #0).
-  Qed.
-  Definition lam : expr := λ: "x", "x" + #21.
+  Proof. intros. rewrite /rec_app. do_step done. Qed.
+  Definition lam : expr [] := (λ: "x", '"x" + #21)%E.
   Goal ∀ σ, prim_step (lam #21)%E σ add σ None.
-  Proof.
-    intros. rewrite /lam. (* FIXME: do_step does not work here *)
-    by eapply (Ectx_step  _ _ _ _ _ []), (BetaS <> "x" ("x" + #21) _ #21).
-  Qed.
+  Proof. intros. rewrite /lam. do_step done. Qed.
 End LangTests.
 
 Section LiftingTests.
@@ -27,8 +21,8 @@ Section LiftingTests.
   Implicit Types P Q : iPropG heap_lang Σ.
   Implicit Types Φ : val → iPropG heap_lang Σ.
 
-  Definition heap_e  : expr :=
-    let: "x" := ref #1 in "x" <- !"x" + #1;; !"x".
+  Definition heap_e  : expr [] :=
+    let: "x" := ref #1 in '"x" <- !'"x" + #1 ;; !'"x".
   Lemma heap_e_spec E N :
      nclose N ⊆ E → heap_ctx N ⊑ || heap_e @ E {{ λ v, v = #2 }}.
   Proof.
@@ -42,16 +36,11 @@ Section LiftingTests.
 
   Definition FindPred : val :=
     rec: "pred" "x" "y" :=
-      let: "yp" := "y" + #1 in
-      if: "yp" < "x" then "pred" "x" "yp" else "y".
+      let: "yp" := '"y" + #1 in
+      if: '"yp" < '"x" then '"pred" '"x" '"yp" else '"y".
   Definition Pred : val :=
     λ: "x",
-      if: "x" ≤ #0 then -FindPred (-"x" + #2) #0 else FindPred "x" #0.
-
-  Instance FindPred_closed : Closed FindPred | 0.
-  Proof. solve_closed. Qed.
-  Instance Pred_closed : Closed Pred | 0.
-  Proof. solve_closed. Qed.
+      if: '"x" ≤ #0 then -^FindPred (-'"x" + #2) #0 else ^FindPred '"x" #0.
 
   Lemma FindPred_spec n1 n2 E Φ :
     n1 < n2 → 
@@ -74,7 +63,7 @@ Section LiftingTests.
   Qed.
 
   Lemma Pred_user E :
-    (True : iProp) ⊑ || let: "x" := Pred #42 in Pred "x" @ E {{ λ v, v = #40 }}.
+    (True : iProp) ⊑ || let: "x" := Pred #42 in ^Pred '"x" @ E {{ λ v, v = #40 }}.
   Proof.
     intros. ewp apply Pred_spec. wp_let. ewp apply Pred_spec. auto with I.
   Qed.
