heap_lang/derived.v
@@ -19,12 +19,12 @@ Implicit Types Φ : val → iProp heap_lang Σ.
 (** Proof rules for the sugar *)
 Lemma wp_lam E x ef e v Φ :
   to_val e = Some v →
-  ▷ || subst' ef x v @ E {{ Φ }} ⊑ || App (Lam x ef) e @ E {{ Φ }}.
+  ▷ || subst' x e ef @ E {{ Φ }} ⊑ || App (Lam x ef) e @ E {{ Φ }}.
 Proof. intros. by rewrite -wp_rec. Qed.
 
 Lemma wp_let E x e1 e2 v Φ :
   to_val e1 = Some v →
-  ▷ || subst' e2 x v @ E {{ Φ }} ⊑ || Let x e1 e2 @ E {{ Φ }}.
+  ▷ || subst' x e1 e2 @ E {{ Φ }} ⊑ || Let x e1 e2 @ E {{ Φ }}.
 Proof. apply wp_lam. Qed.
 
 Lemma wp_seq E e1 e2 v Φ :
@@ -37,17 +37,13 @@ Proof. rewrite -wp_seq // -wp_value //. Qed.
 
 Lemma wp_match_inl E e0 v0 x1 e1 x2 e2 Φ :
   to_val e0 = Some v0 →
-  ▷ || subst' e1 x1 v0 @ E {{ Φ }} ⊑ || Match (InjL e0) x1 e1 x2 e2 @ E {{ Φ }}.
-Proof.
-  intros. rewrite -wp_case_inl // -[X in _ ⊑ X]later_intro. by apply wp_let.
-Qed.
+  ▷ || subst' x1 e0 e1 @ E {{ Φ }} ⊑ || Match (InjL e0) x1 e1 x2 e2 @ E {{ Φ }}.
+Proof. intros. by rewrite -wp_case_inl // -[X in _ ⊑ X]later_intro -wp_let. Qed.
 
 Lemma wp_match_inr E e0 v0 x1 e1 x2 e2 Φ :
   to_val e0 = Some v0 →
-  ▷ || subst' e2 x2 v0 @ E {{ Φ }} ⊑ || Match (InjR e0) x1 e1 x2 e2 @ E {{ Φ }}.
-Proof.
-  intros. rewrite -wp_case_inr // -[X in _ ⊑ X]later_intro. by apply wp_let.
-Qed.
+  ▷ || subst' x2 e0 e2 @ E {{ Φ }} ⊑ || Match (InjR e0) x1 e1 x2 e2 @ E {{ Φ }}.
+Proof. intros. by rewrite -wp_case_inr // -[X in _ ⊑ X]later_intro -wp_let. Qed.
 
 Lemma wp_le E (n1 n2 : Z) P Φ :
   (n1 ≤ n2 → P ⊑ ▷ Φ (LitV (LitBool true))) →
